Make all good pointers be in same frame

Gpointers.fst
@@ -5,25 +5,27 @@ module ST = FStar.HyperStack.ST
 module B = FStar.Buffer
 module CN = C.Nullity
 
+assume val gpointer_frame : (f:Monotonic.HyperHeap.rid{ST.is_eternal_region f})
+
 type gpointer t = (p:C.Nullity.pointer t{
     B.max_length p = 1 /\
     B.idx p = 0 /\
     ~(HS.is_mm (B.content p)) /\
-    ST.is_eternal_region (B.frameOf p)
+    B.frameOf p = gpointer_frame
   })
 
 type gpointer_or_null t = (p:C.Nullity.pointer_or_null t{
     B.max_length p <= 1 /\
     B.idx p = 0 /\
     ~(HS.is_mm (B.content p)) /\
-    ST.is_eternal_region (B.frameOf p)
+    B.frameOf p = gpointer_frame
   })
 
 type gnull t = (p:C.Nullity.pointer_or_null t{
     B.max_length p = 0 /\
     B.idx p = 0 /\
     ~(HS.is_mm (B.content p)) /\
-    ST.is_eternal_region (B.frameOf p)
+    B.frameOf p = gpointer_frame
   })
 
 (** Allow comparing pointers *)
